Bdd/DecisionTree.lean
@@ -36,4 +36,42 @@ lemma usesVar_iff (i : Fin n) (T : DecisionTree n) :
       | inl => simp_all [usesVar.low]
       | inr => simp_all [usesVar.high]
 
+def lift : n ≤ n' → DecisionTree n → DecisionTree n'
+  | _, .leaf b => .leaf b
+  | e, .branch j l h => .branch ⟨j.1, by omega⟩ (lift e l) (lift e h)
+
+lemma lift_injective {n n' : Nat} {h : n ≤ n'} : Function.Injective (lift h) := by
+  intro x y hxy
+  cases x with
+  | leaf _ =>
+    cases y with
+    | leaf _ => simp only [lift] at hxy; simp_all
+    | branch _ _ _ => contradiction
+  | branch _ _ _ =>
+    cases y with
+    | leaf _ => contradiction
+    | branch _ _ _ =>
+      simp only [lift] at hxy
+      injection hxy with a b c
+      rw [lift_injective b, lift_injective c]
+      simp_all only [Fin.mk.injEq, DecisionTree.branch.injEq, and_self, and_true]
+      ext
+      simp_all only
+
+lemma lift_evaluate {h : n ≤ n'} {T : DecisionTree n} {I : Vector Bool n'} :
+    (lift h T).evaluate I = T.evaluate (Vector.cast (show (min n n') = n by simpa) (I.take n)) := by
+  cases T with
+  | leaf => simp [lift, DecisionTree.evaluate]
+  | branch _ _ _ =>
+    simp only [lift, DecisionTree.evaluate]
+    rw [lift_evaluate]
+    rw [lift_evaluate]
+    refine ite_congr ?_ (congrFun rfl) (congrFun rfl)
+    simp only [eq_iff_iff, Bool.coe_iff_coe, Fin.getElem_fin]
+    rename_i a _ _
+    have : (I.take n)[a.1] = I[a.1] := by
+      apply Vector.getElem_take
+    rw [← this]
+    rfl
+
 end DecisionTree
