Bdd/Sim.lean
@@ -11,16 +11,12 @@ structure State (O : OBdd n m) (U : OBdd n m') where
   hl : ∀ j j', lr[j]? = some j' → rl[j']? = some j ∧ Pointer.Reachable O.1.heap O.1.root (.node j)  ∧ ∃ hj : Bdd.Ordered ⟨O.1.heap, .node j⟩, ∃ hj' : Bdd.Ordered ⟨U.1.heap, .node j'⟩, OBdd.HSimilar ⟨⟨O.1.heap, .node j⟩, hj⟩ ⟨⟨U.1.heap, .node j'⟩, hj'⟩
   hr : ∀ j j', rl[j']? = some j → lr[j]? = some j' ∧ Pointer.Reachable U.1.heap U.1.root (.node j') ∧ ∃ hj : Bdd.Ordered ⟨O.1.heap, .node j⟩, ∃ hj' : Bdd.Ordered ⟨U.1.heap, .node j'⟩, OBdd.HSimilar ⟨⟨O.1.heap, .node j⟩, hj⟩ ⟨⟨U.1.heap, .node j'⟩, hj'⟩
 
-def sim_helper (O : OBdd n m) (U : OBdd n m')
-    (p : Pointer m)
-    (hpr : Pointer.Reachable O.1.heap O.1.root p)
-    (hp1 : Bdd.Ordered ⟨O.1.heap, p⟩)
-    (hp2 : OBdd.Reduced O)
-    (q : Pointer m')
-    (hqr : Pointer.Reachable U.1.heap U.1.root q)
-    (hq1 : Bdd.Ordered ⟨U.1.heap, q⟩)
-    (hq2 : OBdd.Reduced U) :
-  StateM (State O U) (Decidable (OBdd.HSimilar ⟨⟨O.1.heap, p⟩, hp1⟩ ⟨⟨U.1.heap, q⟩, hq1⟩)) := do
+def sim_helper
+    (O : OBdd n m) (hO : OBdd.Reduced O)
+    (U : OBdd n m') (hU : OBdd.Reduced U)
+    (p : Pointer m) (hpr : Pointer.Reachable O.1.heap O.1.root p)
+    (q : Pointer m') (hqr : Pointer.Reachable U.1.heap U.1.root q) :
+  StateM (State O U) (Decidable (OBdd.HSimilar ⟨⟨O.1.heap, p⟩, Bdd.ordered_of_reachable hpr⟩ ⟨⟨U.1.heap, q⟩, Bdd.ordered_of_reachable hqr⟩)) := do
   match hp : p with
   | .terminal b =>
     match hq : q with
@@ -40,14 +36,14 @@ def sim_helper (O : OBdd n m) (U : OBdd n m')
         | none =>
           match hr : s.rl[j']? with
           | none =>
-            let hll ← sim_helper O U
-              O.1.heap[j].low (.tail hpr (.low rfl)) (Bdd.ordered_of_reachable (.tail hpr (.low rfl))) hp2
-              U.1.heap[j'].low (.tail hqr (.low rfl)) (Bdd.ordered_of_reachable (.tail hqr (.low rfl))) hq2
+            let hll ← sim_helper O hO U hU
+              O.1.heap[j].low (.tail hpr (.low rfl))
+              U.1.heap[j'].low (.tail hqr (.low rfl))
             match hll with
             | isTrue ht =>
-              let hhh ← sim_helper O U
-                O.1.heap[j].high (.tail hpr (.high rfl)) (Bdd.ordered_of_reachable (.tail hpr (.high rfl))) hp2
-                U.1.heap[j'].high (.tail hqr (.high rfl)) (Bdd.ordered_of_reachable (.tail hqr (.high rfl))) hq2
+              let hhh ← sim_helper O hO U hU
+                O.1.heap[j].high (.tail hpr (.high rfl))
+                U.1.heap[j'].high (.tail hqr (.high rfl))
               match hhh with
               | isTrue ht' =>
                 set
@@ -64,8 +60,8 @@ def sim_helper (O : OBdd n m) (U : OBdd n m')
                           simp only [true_and]
                           constructor
                           · exact hpr
-                          · use hp1
-                            use hq1
+                          · use Bdd.ordered_of_reachable hpr
+                            use Bdd.ordered_of_reachable hqr
                             simp only [OBdd.HSimilar]
                             conv =>
                               lhs
@@ -96,8 +92,8 @@ def sim_helper (O : OBdd n m) (U : OBdd n m')
                           simp only [true_and]
                           constructor
                           · exact hqr
-                          · use hp1
-                            use hq1
+                          · use Bdd.ordered_of_reachable hpr
+                            use Bdd.ordered_of_reachable hqr
                             simp only [OBdd.HSimilar]
                             conv =>
                               lhs
@@ -136,7 +132,7 @@ def sim_helper (O : OBdd n m) (U : OBdd n m')
               simp only [OBdd.HSimilar] at contra h5
               rw [← contra] at h5
               rcases s.hl i j' h1 with ⟨h1', h2', h3', h4', h5'⟩
-              have := @hp2.2 ⟨(Pointer.node i), h2'⟩ ⟨(Pointer.node j), hpr⟩ h5
+              have := @hO.2 ⟨(Pointer.node i), h2'⟩ ⟨(Pointer.node j), hpr⟩ h5
               simp [InvImage] at this
               subst this
               rw [h1] at hl
@@ -156,17 +152,26 @@ def sim_helper (O : OBdd n m) (U : OBdd n m')
               simp only [OBdd.HSimilar] at c h5
               rw [c] at h5
               rcases s.hr j i' h1 with ⟨h1', h2', h3', h4', h5'⟩
-              have := @hq2.2 ⟨.node j', hqr⟩ ⟨.node i', h2'⟩ h5
+              have := @hU.2 ⟨.node j', hqr⟩ ⟨.node i', h2'⟩ h5
               simp [InvImage] at this
               exact this
             ))
       | isFalse hvf => return isFalse (fun c ↦ by simp [OBdd.HSimilar, OBdd.toTree_node] at c; exact hvf c.1)
-termination_by OBdd.size' (⟨⟨O.1.heap, p⟩, hp1⟩ : OBdd n m)
+termination_by OBdd.size' (⟨⟨O.1.heap, p⟩, Bdd.ordered_of_reachable hpr⟩ : OBdd n m)
 decreasing_by
   · simp [OBdd.size_node, OBdd.low, Bdd.low]; omega
   · simp [OBdd.size_node, OBdd.high, Bdd.high]
 
-instance instDecidableRobddHSimilar (O : OBdd n m) (hO : O.Reduced) (U : OBdd n m') (hU : U.Reduced) : Decidable (O.HSimilar U) :=
-  ((sim_helper O U O.1.root .refl O.2 hO U.1.root .refl U.2 hU) ⟨Std.HashMap.emptyWithCapacity 0, Std.HashMap.emptyWithCapacity 0, by simp, by simp⟩).1
+instance instDecidableRobddHSimilar
+    (O : OBdd n m) (hO : O.Reduced)
+    (U : OBdd n m') (hU : U.Reduced) :
+    Decidable (O.HSimilar U) :=
+  ((sim_helper O hO U hU O.1.root .refl U.1.root .refl)
+    ⟨ Std.HashMap.emptyWithCapacity 0,
+      Std.HashMap.emptyWithCapacity 0,
+      by simp,
+      by simp
+    ⟩
+  ).1
 
 end Sim
